\begin{sol}
        \begin{enumerate}[label=\textbf{(\alph*)}]
            \item
            The rotation operator can be expanded into its series
            \[
                R_\epsilon(\mathbf{n})=\exp\left(- i\epsilon\mathbf{n}\cdot\mathbf{S} \right)=1-i\epsilon\mathbf{n}\cdot\mathbf{S}+\mathcal{O}\left( \epsilon^2 \right) \:\:\:\:\:\: 
                R_\epsilon^\dagger(\mathbf{n})=\exp\left( -i\epsilon\mathbf{n}\cdot\mathbf{S} \right)=1+i\epsilon\mathbf{n}\cdot\mathbf{S}+\mathcal{O}\left( \epsilon^2 \right)  
            \]
            \[
                R_\epsilon^\dagger(\mathbf{n})\mathbf{S}R_\epsilon^\dagger(\mathbf{n})=\mathbf{S}+i\epsilon\mathbf{n\cdot S}\mathbf{S}-i\epsilon\mathbf{Sn\cdot S}
            \] 
            \[
                =\mathbf{S}+i\epsilon[\mathbf{n\cdot S},\mathbf{S}]=\mathbf{S}+\epsilon(\mathbf{n}\times\mathbf{S})
            \] 
        \item
            \[
                \bra{\mathbf{n'};+}R_\epsilon^\dagger(\mathbf{n})\mathbf{S}R_\epsilon(\mathbf{n})\ket{\mathbf{n'};+} = 
            .\] 

        \end{enumerate}
    \end{sol}    