\begin{sol}
\begin{enumerate}[label=\textbf{(\alph*)}]
\item
Given $u_k=Av_k$ and $v_k=Bu_k$, the matrix representation of A is $u_j=A_{ij} v_i$ and the matrix representation of B is $v_j=B_{ij}u_i$. 
\\A and B are inverses since $ABu_k=A(Bu_k)=Av_k=u_k$ and $BAv_k=B(Av_k)=Bu_k=v_k$. Thus, $AB=BA=\mathbf{1}$, so $B=A^{-1}$ by definition.
\item
Using change of basis for matrices, $T_{ij}(\{u\})=A^{-1}T_{ij}(\{v\})A, T_{ij}(\{v\})=AT_{ij}(\{u\})A^{-1}$.
\item
Note the property of the identity $\mathbf{1}_{ij}=\delta_{ij}$. Thus, $A^{-1}_{ij}A_{jk}=A_{jk}A^{-1}_{ij}=\delta_{ik}$.
$$tr(T\{u\})\equiv T\{u\}_{ii}=(A^{-1}T\{v\}A)_{ii}$$ 
$$=A^{-1}_{ij}T\{v\}_{jk}A_{ki}=A^{-1}_{ij}A_{ki}T\{v\}_{jk}=\delta_{jk}T\{v\}_{jk}$$   
$$=T\{v\}_{jj}\equiv tr(T\{v\})$$  
\item
Using the identity $\det(AB)=\det(A)\det(B)$
$$\det(T\{u\})=\det(A^{-1}T\{v\}A)=\det(A^{-1})\det(T\{v\})\det(A)$$
$$=\det(A^{-1}A)\det(T\{v\})=\det(\mathbf{1})\det(T\{v\})=\det(T\{v\})$$ 

\end{enumerate}
\end{sol}