\begin{sol}
It has been derived that the equation for the Heisenberg operator is
\begin{equation}
	\frac{d\hat A_H}{dt}=\frac{\partial \hat A_S}{\partial t}-i[\hat A_H,\hat H_H]
\end{equation}
Since the Schrodinger operators $\hat S_x,\hat S_y,\hat S_z$ are time-independent, therefore
\begin{equation}
	\frac{d\hat A_H}{dt}=-i[\hat A_H,\hat H_H]
\end{equation}
The time evolution of Heisenberg operator for $S_z$ is trivial since it commutes with the Hamiltonian. Thus, the it is time independent and it is equal to the Schrodinger operator.\\
It is known that the commutators
\begin{equation}
	[\hat S_i,\hat S_j]=i\epsilon_{ijk}\hat S_k
\end{equation} 
Thus,
\begin{equation}
	\frac{d(\hat S_x)_H}{dt}=-i[\hat S_x,\hat H]=i\lambda B[\hat S_x,\hat S_z]=\lambda B\hat S_y
\end{equation}
\begin{equation}
	\frac{d(\hat S_y)_H}{dt}=-i[\hat S_y,\hat H]=i\lambda B[\hat S_y,\hat S_z]=-\lambda B\hat S_x
\end{equation}
Solving the differential equations with the initial conditons that $(\hat S_x)_H(0)=\hat S_x$ and $(\hat S_y)_H(0)=\hat S_y$. The Heisenberg operators can be obtained.
\begin{equation}
	(\hat S_x)_H=\hat S_x+\lambda Bt\hat S_y\:\:\:\:\:\:\:\:(\hat S_y)_H=\hat S_y-\lambda Bt\hat S_x\:\:\:\:\:\:\:\:\:(\hat S_z)_H=S_y
\end{equation} 

\end{sol}