\begin{sol}
\begin{enumerate}[label=\textbf{(\alph*)}]
\item
The Hamiltonian of the shifted harmonic oscillator is 
$$\hat H=\frac{\hat p^2}{2m}+\frac{1}{2}m\omega^2\hat x^2-F\hat x$$
Complete the square for the second and third terms of the Hamiltonian. Let a characteristic length $\beta\equiv\frac{F}{m\omega^2}$
$$\hat H=\frac{p^2}{2m}+\frac{1}{2}m\omega^2(\hat x-\beta)^2-\frac{1}{2}m\omega^2\beta^2$$
Define a new position operator $\hat y\equiv \hat x-\beta$. The Hamiltonian can be rewritten as
$$\hat H=\frac{p^2}{2m}+\frac{1}{2}m\omega^2\hat y^2-\frac{1}{2}m\omega^2\beta^2$$
It is clear that this Hamiltonian is analogous to the Hamiltonian of the normal simple harmonic oscillator with $\hat y$ being the position operator. For a simple harmonic oscillator, the expectation value of the position in the ground state is zero. Thus, $\langle\hat y\rangle=0$. 
$$\langle x\rangle=\langle y\rangle-\beta=-\frac{F}{m\omega^2}$$
\item
Define the operator
$$\hat a_y\equiv\sqrt{\frac{m\omega}{2}}\left(\hat y+\frac{i\hat p}{m\omega}\right)=\hat a-\sqrt{\frac{m\omega}{2}}\beta$$
This is the annihilation operator of the shifted harmonic oscillator. Thus, $\hat a_y\ket {0'}=0$.
It is given that 
$$\ket{0'}=Ne^{\alpha \hat a^\dagger}\ket 0$$
For simplicity, let $\gamma\equiv\sqrt{\frac{m\omega}{2}}\beta$ 
$$\hat a_y\ket{0'}=(\hat a-\gamma)Ne^{\alpha \hat a^\dagger}\ket 0=0$$ 
Since $N$ is a constant, it can be ignored. Rearranging the terms will result in
$$\hat ae^{\alpha\hat a^\dagger}\ket 0=\gamma e^{\alpha\hat a^\dagger}\ket 0$$
Note that $[\hat a,e^{\alpha\hat a^\dagger}]\ket 0=\hat ae^{\alpha\hat a^\dagger}\ket 0+e^{\alpha\hat a^\dagger}\hat a\ket 0=\hat ae^{\alpha\hat a^\dagger}\ket 0$. Hence, $[\hat a,e^{\alpha\hat a^\dagger}]\ket 0=\gamma e^{\alpha\hat a^\dagger}\ket 0$.\\
It will be helpful to compute the commutator. First, use the definition of the exponential and the linearity of the commutator.
$$[\hat a,e^{\alpha\hat a^\dagger}]=\sum_{n=0}^\infty\frac{\alpha^n}{n!}[a,(a^\dagger)^n]$$
It was computed in \textit{5b, p.52} that $[a,(a^\dagger)^n]=n(a^\dagger)^{n-1}$ for $n\geq 1$. Note that $a$ commutes with $(a^\dagger)^0$ which is the identity operator.
$$[\hat a,e^{\alpha\hat a^\dagger}]=\sum_{n=1}^\infty\frac{\alpha^n}{n!}[a,(a^\dagger)^n]=\sum_{n=1}^\infty\frac{\alpha^n}{n!}n(a^\dagger)^{n-1}=\sum_{n=1}^\infty\frac{\alpha^n(a^\dagger)^{n-1}}{(n-1)!}=\alpha\sum_{j=0}^\infty\frac{\alpha^j(a^\dagger)^{j}}{j!}=\alpha e^{\alpha \hat a^\dagger}$$ 
Substituting this result in the previous expression will yield
$$[\hat a,e^{\alpha\hat a^\dagger}]\ket 0=\alpha e^{\alpha\hat a^\dagger}\ket 0=\gamma e^{\alpha\hat a^\dagger}\ket 0$$
$$\alpha=\gamma=\sqrt{\frac{m\omega}{2}}\frac{F}{m\omega^2}=\frac{F}{\sqrt{2m\omega^3}}$$ 

\end{enumerate}
\end{sol}