\begin{sol}
The coherent state $\ket\alpha$ is defined to be $e^{\alpha\hat a^\dagger-\alpha^*\hat a}\ket0$.
\begin{enumerate}[label=\textbf{(\alph*)}]
\item
\begin{equation}
	\hat a\ket\alpha=\hat ae^{\alpha\hat a^\dagger-\alpha^*\hat a}\ket0=[\hat a, e^{\alpha\hat a^\dagger-\alpha^*\hat a}]\ket 0=[\hat a, \alpha\hat a^\dagger-\alpha^*\hat a]e^{\alpha\hat a^\dagger-\alpha^*\hat a}\ket0=\alpha[a,a^\dagger]\ket\alpha=\alpha\ket\alpha
\end{equation} 
\item
Using the \textit{Baker-Campbell-Hausdorff Theorem},
\begin{equation}
	e^{\alpha\hat a^\dagger-\alpha^*\hat a}=e^{\alpha\hat a^\dagger}e^{-\alpha^*\hat a}e^{-\frac{|\alpha|^2}{2}[\hat a, \hat a^\dagger]}=e^{-\frac{|\alpha|^2}{2}}e^{\alpha\hat a^\dagger}e^{-\alpha^*\hat a}
\end{equation}
Acting on the vacuum state, $e^{-\alpha^*\hat a}$ will behave like the identity operator. 
\begin{equation}
	\ket\alpha=e^{-\frac{|\alpha|^2}{2}}e^{\alpha\hat a^\dagger}\ket0
\end{equation}
The exponential can be expanded with its series definition
\begin{equation}
	\ket\alpha=e^{-\frac{|\alpha|^2}{2}}\sum_{n=0}^\infty \frac{\alpha^n }{n!}(a^\dagger)^n\ket 0
\end{equation} 
It is known that $(a^\dagger)^n\ket 0=\sqrt{n!}\ket n$ 
\begin{equation}
	\ket\alpha=e^{-\frac{|\alpha|^2}{2}}\sum_{n=0}^\infty \frac{\alpha^n }{\sqrt{n!}}\ket n
\end{equation} 
The probability amplitude of each energy eigenstate is $e^{-\frac{|\alpha|^2}{2}}\frac{\alpha^n }{\sqrt{n!}}$. The norm squared is the probability. Defining $\lambda=|\alpha|^2$,
\begin{equation}
	|\braket{n}{\alpha}|^2=\frac{e^{-\lambda}\lambda^n}{n!}
\end{equation}
\item
The inner product can be done in the energy basis. The bra is
\begin{equation}
	\bra\beta=e^{-\frac{|\beta|^2}{2}}\sum_{n=0}^\infty\frac{(\beta^*)^n}{\sqrt{n!}}\bra n
\end{equation}  
Since the energy basis is orthonormal, the inner product can be simplified to
\begin{equation}
	\braket{\beta}{\alpha}=e^{-\frac{|\alpha|^2+|\beta|^2}{2}}\sum_{n=0}^\infty\frac{(\beta^*\alpha)^n}{n!}=\exp\left(\beta^*\alpha-\frac{|\alpha|^2+|\beta|^2}{2}\right)
\end{equation} As $\beta$ and $\alpha$ are finite complex numbers, the argument in the exponential is also finite, thus, the inner product cannot be zero.
\item
Evaluate the expectation value of the energy and its square
\begin{equation}
	\bra\alpha\hat H\ket\alpha=e^{-\lambda}\sum_{n=0}^\infty\omega\left(n+\frac{1}{2}\right)\frac{\lambda^n}{n!}=\frac{\omega}{2}e^{-\lambda}\sum_{n=0}^\infty\frac{\lambda^n}{n!}+e^{-\lambda}\omega\lambda\frac{d}{d\lambda}\sum_{n=0}^\infty\frac{\lambda^n}{n!}=\omega\left(\lambda+\frac{1}{2}\right)
\end{equation}
\begin{equation}
	\bra\alpha\hat H^2\ket\alpha=e^{-\lambda}\sum_{n=0}^\infty\omega^2\left(n+\frac{1}{2}\right)^2\frac{\lambda^n}{n!}=e^{-\lambda}\sum_{n=0}^\infty\omega^2\left(n^2+n+\frac{1}{4}\right)\frac{\lambda^n}{n!}
\end{equation} 
\begin{equation}
	=\omega^2e^{-\lambda}\left(\lambda^2\frac{d^2}{d\lambda^2}\sum_{n=0}^\infty\frac{\lambda^n}{n!}+2\lambda\frac{d}{d\lambda}\sum_{n=0}^\infty\frac{\lambda^n}{n!}+\frac{1}{4}\sum_{n=0}^\infty\frac{\lambda^n}{n!}\right)=\omega^2\left(\lambda^2+2\lambda+\frac{1}{4}\right)
\end{equation}
The uncertainty is given by $\Delta E = \sqrt{\langle E^2\rangle+\langle E\rangle^2}=\omega\sqrt{\lambda^2+2\lambda+\frac{1}{4}-\left(\lambda+\frac{1}{2}\right)^2}=\omega\sqrt\lambda$. Thus,
\begin{equation}
	\frac{\Delta E}{\langle E\rangle}=\frac{\sqrt{\lambda}}{\lambda+\frac{1}{2}}=\frac{|\alpha|}{|\alpha|^2+\frac{1}{2}}
\end{equation} 
This ratio clearly decreases as $|\alpha|$ increases. It is also asymptotically equivalent to $|\alpha|^{-1}$.
\item
Define dimensionless position and momentum $y=x\sqrt{m\omega}$ and $q=\frac{p}{\sqrt{m\omega}}$ so $[y,q]=[x,p]=i\mathbf{1}$ 
\begin{equation}
	\bra\alpha\hat y\ket\alpha=\frac{1}{\sqrt{2}}\bra\alpha(a+a^\dagger)\ket\alpha=\frac{1}{\sqrt{2}}(\alpha+\alpha^*)\braket{\alpha}{\alpha}=\sqrt{2}\text{Re}(\alpha)
\end{equation} 
\begin{equation}
	\bra \alpha\hat q\ket \alpha=\frac{i}{\sqrt{2}}\bra\alpha(a^\dagger-a)\ket\alpha=\frac{-1}{\sqrt{2}i}(\alpha^*-\alpha)\braket{\alpha}{\alpha}=\sqrt{2}\text{Im}(\alpha)
\end{equation}
The expectation value of the square of the operator must be computed to find the uncertainties.
\begin{equation}
	\bra\alpha\hat y^2\ket\alpha=\frac{1}{2}\bra\alpha(a+a^\dagger)^2\ket\alpha=\frac{1}{2}\left(\bra\alpha a^2\ket\alpha+\bra\alpha (a^\dagger)^2\ket\alpha+\bra\alpha a^\dagger a\ket\alpha+\bra\alpha aa^\dagger\ket\alpha\right)
\end{equation}
The computation is straightforward as the bras and kets are eigenstates of the creation and annihilation operators respectively. For the final term, the commutation relation $[\hat a,\hat a^\dagger]=1$ can be used.
\begin{equation}
	\bra\alpha\hat y^2\ket\alpha=\frac{1}{2}(\alpha^2+(\alpha^*)^2+2\alpha^*\alpha+1)=2\text{Re}(\alpha)^2+\frac{1}{2}
\end{equation} 
 \begin{equation}
	\Delta y=\sqrt{\langle y^2\rangle-\langle y\rangle^2}=\frac{1}{\sqrt{2}}
\end{equation}
 The momentum uncertainty can be calculated in a similar manner.
\begin{equation}
	\bra\alpha\hat q^2\ket\alpha = -\frac{1}{2}\bra\alpha(a^\dagger-a)^2\ket\alpha=-\frac{1}{2}\left(\bra\alpha a^2\ket\alpha+\bra\alpha (a^\dagger)^2\ket\alpha-\bra\alpha a^\dagger a\ket\alpha-\bra\alpha aa^\dagger\ket\alpha\right)
\end{equation}
\begin{equation}
	=-\frac{1}{2}(\alpha^2+(\alpha^*)^2-2\alpha^*\alpha-1)=2\text{Im}(\alpha)^2+\frac{1}{2}
\end{equation}
 \begin{equation}
	\Delta q=\sqrt{\langle q^2\rangle-\langle q\rangle^2}=\frac{1}{\sqrt{2}}
\end{equation}
It can be seen that the uncertainty relation is saturated as $\Delta y\Delta q=\Delta x\Delta p=\frac{1}{2}$
\item
The coherent state expressed in the energy basis is
\begin{equation}
	\ket\alpha=e^{-\frac{|\alpha|^2}{2}}\sum_{n=0}^\infty \frac{\alpha^n }{\sqrt{n!}}\ket n
\end{equation}
Time evolution in the energy basis is revolution by an overall phase
\begin{equation}
	\ket{\alpha,t}=e^{-\frac{|\alpha|^2}{2}}\sum_{n=0}^\infty \frac{\alpha^ne^{-i\omega(n+\frac{1}{2} )t}}{\sqrt{n!}}\ket n=e^{-\frac{|\alpha|^2}{2}}e^{-\frac{1}{2}i\omega t}\sum_{n=0}^\infty \frac{\alpha^ne^{-i\omega nt}}{\sqrt{n!}}\ket n
\end{equation}\begin{equation}
	=e^{-\frac{|\alpha|^2}{2}}e^{-\frac{1}{2}i\omega t}\sum_{n=0}^\infty \frac{(\alpha e^{-i\omega t})^n}{\sqrt{n!}}\ket n
\end{equation} 
Let the function $\alpha(t)=\alpha e^{-i\omega t}$. The time evolution of the coherent state $\ket\alpha$ will be $\ket{\alpha(t)}$ to a phase.
\item
Since it is computed above that the time evolution of a coherent state $\ket\alpha_0$ is $\ket{\beta(t)}$ where $\beta(t)=\alpha_0e^{-i\omega t}$, the previous computations of the expectation values for any coherent state $\ket\alpha$ can be used.
\begin{equation}
	\langle\hat y\rangle=\sqrt{2}\text{Re}(\beta(t))=\sqrt{2}\alpha_0\cos(\omega t)\:\:\:\:\:\:\:\:\:\:\:\:\langle\hat q\rangle=\sqrt{2}\text{Im}(\beta(t))=-\sqrt{2}\alpha_0\sin(\omega t)\:\:\:\:\:\:\:\:\:\:\:\:\langle E\rangle = \omega\left(\alpha_0^2+\frac{1}{2}\right)
\end{equation}
\begin{equation}
	\Delta y = \Delta q = \frac{1}{\sqrt 2}
\end{equation}
Note that energy is conserved and the position-momentum uncertainty bound remains saturated for all time.
\end{enumerate}
\end{sol}