\begin{sol}
Show $\Omega\ket\Psi=\langle\Omega\rangle\ket\Psi+(\Delta\Omega){\ket\Psi_\perp}\implies\braket{\Psi_\perp}{\Psi_\perp}=1,\braket{\Psi}{\Psi_\perp}=0$\\\\
The proof of the second statement is done by operating on both sides with the operator $\bra\Psi$ to get
\begin{equation}
	\bra\Psi\Omega\ket\Psi=\langle\Omega\rangle\braket{\Psi}{\Psi}+(\Delta\Omega)\braket{\Psi}{\Psi_\perp}
\end{equation}
By definition of the expectation value, $\bra\Psi\Omega\ket\Psi\equiv\langle\Omega\rangle\braket{\Psi}{\Psi}$, thus $(\Delta\Omega)\braket{\Psi}{\Psi_\perp}=0$. Since it is given the uncertainty is non-zero, $\braket{\Psi}{\Psi_\perp}=0$.

\end{sol}