\begin{sol}
Notice the following about the matrix $\mathbf{M}$.
\begin{equation}
	\mathbf{MM}=\begin{pmatrix}0 & -i\\i&0\end{pmatrix}\begin{pmatrix}0 & -i\\i&0\end{pmatrix}=\begin{pmatrix}
1&0\\0&1
\end{pmatrix}\equiv\mathbf{1}
\end{equation} 
By definition, $\mathbf{1M}\equiv\mathbf{M}$ and $\mathbf{M}^1=\mathbf{M}$, it can be deduced by induction from $\mathbf{MM}=\mathbf{1}$ that
\begin{equation}
	\mathbf{M}^{2n}=\mathbf{1} \text{ and } \mathbf{M}^{2n+1}=\mathbf{M}\text{ for }n\in\mathbb{Z}
\end{equation}

Take the taylor expansion of $e^{iM\theta}$
\begin{equation}
	e^{iM\theta}=\sum_{n=0}^\infty\frac{i^n(\mathbf{M}\theta)^n}{n!}=1+i\mathbf{M}\theta-\frac{(\mathbf{M}\theta)^2}{2}-\frac{i(\mathbf{M}\theta)^3}{6}...
\end{equation} 
\begin{equation}
	=\sum_{n=0}^\infty(-1)^n\frac{\mathbf{M}^{2n}\theta^{2n}}{(2n)!}+i\sum_{n=0}^\infty(-1)^n\frac{\mathbf{M}^{2n+1}\theta^{2n+1}}{(2n+1)!}
\end{equation}
\begin{equation}
	=\mathbf{1}\sum_{n=0}^\infty(-1)^n\frac{\theta^{2n}}{(2n)!}+i\mathbf{M}\sum_{n=0}^\infty(-1)^n\frac{\theta^{2n+1}}{(2n+1)!}
\end{equation}
\begin{equation}
	=\cos(\theta)\mathbf{1}+i\sin(\theta)\mathbf{M}
\end{equation}
The algebraic property of any matrix that would lead to this result is the matrix is its own inverse.
\end{sol}