\begin{sol}
\begin{enumerate}[label=\textbf{(\alph*)}]
  \item 
  \begin{equation}
    \hat{p}\psi=-i\frac{d}{dx}\psi=-ie^{i\alpha}\phi'
  \end{equation}
  \begin{equation}
    \begin{aligned}
      \langle\hat{p}\rangle&=\bra{\psi}\hat{p}\ket{\psi}=-i\int_{-\infty}^{\infty}\phi(x)\phi'(x)dx=-i[\phi(x)^2]_{-\infty}^{\infty}+i\int_{-\infty}^{\infty}\phi(x)\phi'(x)dx\\
      &=2\int_{-\infty}^{\infty}\phi(x)\phi'(x)dx=[\phi(x)^2]_{-\infty}^{\infty}
    \end{aligned}
  \end{equation}
      
  Since $\phi(x)$ must vanish at $-\infty$ and $\infty$
  \begin{equation}
    \int_{-\infty}^{\infty}\phi(x)\phi'(x)dx=0
  \end{equation}
  \begin{equation}
    \langle\hat{p}\rangle=0
  \end{equation}
    \item
    \begin{equation}
      \hat{p}\psi=-i\partial_x\psi=-i(\phi_1'+e^{i\alpha}\phi_2')
    \end{equation}
    \begin{equation}
      \begin{aligned}
        \langle\hat{p}\rangle&=\bra{\psi}\hat{p}\ket{\psi}=-i\int_{-\infty}^{\infty}(\phi_1 (x)+e^{-i\alpha}\phi_2(x))(\phi_1'(x)+e^{i\alpha}\phi_2'(x))dx\\
        &=-ie^{-i\alpha}\int_{-\infty}^{\infty}\phi_1'(x)\phi_2(x)dx-ie^{i\alpha}\int_{-\infty}^{\infty}\phi_1(x)\phi_2'(x)dx
      \end{aligned}
    \end{equation}

Using integration by parts on the second term will yield
\begin{equation}
  -ie^{i\alpha}\int_{-\infty}^{\infty}\phi_1(x)\phi_2'(x)dx=-ie^{i\alpha}[\phi_1(x)\phi_2(x)]_{-\infty}^{\infty}+ie^{i\alpha}\int_{-\infty}^{\infty}\phi_1'(x)\phi_2(x)dx
\end{equation}

Since both $\phi_1(x)$ and $\phi_2(x)$ must vanish at $-\infty$ and $\infty$, this term becomes 
\begin{equation}
  ie^{i\alpha}\int_{-\infty}^{\infty}\phi_1'(x)\phi_2(x)dx
\end{equation}

Substituting this term into the expression,  
\begin{equation}
  \langle\hat{p}\rangle=i(e^{i\alpha}-e^{-i\alpha})\int_{-\infty}^{\infty}\phi_1'(x)\phi_2(x)dx
\end{equation}

It is trivial to see that $\langle\hat{p}\rangle=0$ when $e^{i\alpha}=e^{-i\alpha}$. This is true when $\alpha$ is a integer multiple of $\pi$.
\item 
\begin{equation}
  \hat{p}\psi=-i\partial_x\psi=k\phi-ie^{ikx}\phi'
\end{equation} 
\begin{equation}
  \langle\hat{p}\rangle=\bra{\psi}\hat{p}\ket{\psi}=k\braket{\phi}{\phi}-i\braket{\phi}{e^{ikx}\phi'}
\end{equation}

The first term evaluates to k, the second term can be evaluated in a similar manner to part (a):
\begin{equation}
  -i\braket{\phi}{e^{ikx}\phi'}=-i\int_{-\infty}^{\infty}e^{ikx}\phi(x)\phi'(x)dx=-i[e^{ikx}\phi(x)^2]_{-\infty}^{\infty}+i\int_{-\infty}^{\infty}e^{ikx}\phi(x)\phi'(x)dx
\end{equation}
Since $\phi(x)$ must vanish at infinity, $e^{ikx}\phi(x)$ must also vanish at infinity, as $|e^{ikx}|=1\forall x\in\mathbb{R}$. Thus, this integral evaluates to zero.
\begin{equation}
  2\int_{-\infty}^{\infty}e^{ikx}\phi(x)\phi'(x)dx=[e^{ikx}\phi(x)^2]_{-\infty}^{\infty}=0
\end{equation}
The only contributing term to $\langle\hat{p}\rangle$ is the first term. Thus, $\langle\hat{p}\rangle=k$
\end{enumerate}
\end{sol}