\begin{sol}
\begin{enumerate}[label=\textbf{(\alph*)}]
\item

\begin{equation}
	\sum_{a'}|\bra a\hat x\ket{a'}|^2(E_{a'}-E_a)=\sum_{a'}\bra a\hat x\ketbra {a'}{a'}\hat x\ket{a}(E_{a'}-E_a)
\end{equation}
\begin{equation}
	=\bra a\hat x\sum_{a'}E_{a'}\ketbra{a'}{a'}\hat x\ket a-E_{a}\bra a\hat x\sum_{a'}\ketbra{a'}{a'}\hat x\ket a
\end{equation}
From completeness, note the following:
\begin{equation}
	\sum_{a'}\ketbra{a'}{a'}=\mathbf{1}\text{ and }\sum_{a'}E_{a'}\ketbra{a'}{a'}=\hat H
\end{equation} 
The sum can be rewritten in terms of single matrix elements
\begin{equation}
	\sum_{a'}|\bra a\hat x\ket{a'}|^2(E_{a'}-E_a)=\bra a\hat x\hat H\hat x\ket a-E_a\bra a\hat x^2\ket a
\end{equation}

Consider the commutator $[[\hat x,\hat H],\hat x]$
\begin{equation}
	[[\hat x,\hat H],\hat x]=[\hat x,\hat H]\hat x-\hat x[\hat x,\hat H]=\hat x\hat H\hat x-\hat H\hat x^2-\hat x^2\hat H+\hat x\hat H\hat x=2\hat x\hat H\hat x-\{\hat x^2,\hat H\}
\end{equation} 
Evaluate this commutator on the state $\ket a$ will yield
\begin{equation}
	\bra a 2\hat x\hat H\hat x\ket a-\bra a\hat x^2\hat H\ket a-\bra a\hat H\hat x^2\ket a=2\bra a \hat x\hat H\hat x\ket a-2E_a\bra a\hat x^2\ket a
\end{equation}
\begin{equation}
	=2\sum_{a'}|\bra a\hat x\ket{a'}|^2(E_{a'}-E_a)
\end{equation} 
Evaluate the commutator with respect to the position and momentum operators
\begin{equation}
	[[\hat x,\hat H],\hat x]=\frac{1}{2m}[[\hat x,\hat p^2],\hat x]=\frac{1}{2m}[[\hat x,\hat p]\hat p+\hat p[\hat x,\hat p],\hat x]=\frac{i}{m}[\hat p,\hat x]=\frac{1}{m}
\end{equation}   
Therefore,
\begin{equation}
	\sum_{a'}|\bra a\hat x\ket{a'}|^2(E_{a'}-E_a)=\frac{1}{2m}
\end{equation}
\item
Consider the matrix elements of $[\hat H,\hat x]$
\begin{equation}
	\bra a[\hat H,\hat x]\ket {a'}=\bra a\hat H\hat x\ket{a'}-\bra a\hat x\hat H\ket {a'}=(E_a-E_{a'})\bra a\hat x\ket {a'}
\end{equation} 
Evaluate the commutator with respect to the position and momentum operators
\begin{equation}
	[\hat H,\hat x]=-[\hat x,\hat H]=\frac{\hat p}{im}
\end{equation}
The identity can be established
\begin{equation}
	\bra a[\hat H,\hat x]\ket {a'}=\bra a\frac{\hat p}{im}\ket a'=(E_a-E_{a'})\bra a\hat x\ket {a'}
\end{equation}
\begin{equation}
	\bra a\hat p\ket {a'}=im(E_a-E_{a'})\bra a\hat x\ket{a'}
\end{equation} 
Take the norm square of the previous identity
\begin{equation}
	\bra a\hat p\ketbra{a'}\hat p\ket a=(-im(E_a-E_{a'})\bra a\hat x\ket{a'})(im(E_a-E_{a'})\bra {a'}\hat x\ket{a})
\end{equation}
\begin{equation}
	\bra a\hat p\ketbra{a'}\hat p\ket a=m^2(E_a-E_{a'})^2|\bra a\hat x\ket{a'}|^2
\end{equation} 
Moving the factor of $m^2$ to the left and summing over all $a'$ will result in
\begin{equation}
	\frac{1}{m^2}\sum_{a'}\bra a\hat p\ketbra{a'}\hat p\ket a=\sum_{a'}|\bra a\hat x\ket{a'}|^2(E_a-E_{a'})^2
\end{equation} 
Flipping the equation and using completeness yields
\begin{equation}
	\sum_{a'}|\bra a\hat x\ket{a'}|^2(E_a-E_{a'})^2=\frac{\bra a\hat p^2\ket a}{m^2}
\end{equation}
\item
Consider the expectation value of the following commutator on a stationary state $[\hat x\hat p,\hat H]$. For stationary states, the value of any commutator with the Hamiltonian must be zero by definition. Next, rewrite the commutator as
\begin{equation}
	[\hat x\hat p, \hat H]=\frac{[\hat x\hat p,\hat p^2]}{2m}+[\hat x\hat p,V(\hat x)]=0
\end{equation}
Note this equality is only true for stationary states. Next, compute the terms separately, the first term can be simplified
\begin{equation}
	\frac{1}{2m}(\hat x\hat p\hat p\hat p-\hat p\hat p\hat x\hat p)=\frac{[\hat x,\hat p^2]}{2m}\hat p
\end{equation} 
The commutator $[\hat x,\hat p^2]$ was already computed to be $2i\hat p$, thus,
\begin{equation}
	\frac{[\hat x\hat p,\hat p^2]}{2m}=i\frac{\hat p^2}{m}
\end{equation}
The second term can be evaluated using the position-space representation of the momentum operator, $\hat p=-i\nabla$. 
\begin{equation}
	[\hat x\hat p,V(\hat x)]=\hat x\hat p V(\hat x)-V(\hat x)\hat x\hat p=\hat x(-i\nabla)V(\hat x)-V(\hat x)\hat x(-i\nabla)
\end{equation}
\begin{equation}
	=-i\hat x(\nabla V(\hat x)+V(\hat x)\nabla-V(\hat x)\nabla)=-i\hat x\nabla V(\hat x)
\end{equation}
For convenience, both sides of the original equation can be divided by 2 to yield
\begin{equation}
	\frac{1}{2}[\hat x\hat p, \hat H]=i\left(\frac{\hat p^2}{2m}-\frac{1}{2}\hat x\nabla V(\hat x)\right)=0
\end{equation}
Therefore, given a stationary state $\ket a$,
\begin{equation}
	\bra a\frac{\hat p^2}{2m}=\frac{1}{2}\bra a\hat x\nabla V(\hat x)\ket a
\end{equation}
Or, for all stationary states in time-independent potentials,
\begin{equation}
	2\langle T\rangle=\langle x\nabla V\rangle
\end{equation} 
This theorem can be applied for the cases $V(x)=\alpha x^n$. Here,
\begin{equation}
	\langle T\rangle=\frac{\alpha(n-1)}{2}\langle x^n\rangle
\end{equation} 
\end{enumerate}
\end{sol}