\begin{sol}
\begin{enumerate}[label=\textbf{(\alph*)}]
\item
Define $G(t)\equiv e^{t(A+B)}e^{-tA}$,
\begin{equation}
	G^{-1}(t)=e^{tA}e^{-t(A+B)}
\end{equation}
\begin{equation}
	\frac{d}{dt}G(t)=e^{t(A+B)}(A+B)e^{-tA}-e^{t(A+B)}Ae^{-tA}=e^{t(A+B)}Be^{-tA}
\end{equation}
\begin{equation}
	G^{-1}\frac{d}{dt}G(t)=e^{tA}e^{-t(A+B)}e^{t(A+B)}Be^{-tA}=e^{tA}Be^{-tA}
\end{equation}
Using Lemma 8, 
\begin{equation}
	G^{-1}\frac{d}{dt}G(t)=B+ct
\end{equation} 
\item
\begin{equation}
	G(t)=G(0)e^{tB}e^{\frac{1}{2}ct^2}
\end{equation}
\begin{equation}
	\frac{d}{dt}G(t)=G(0)(Be^{tB}e^{\frac{1}{2}ct^2}+e^{tB}ct\,e^{\frac{1}{2}ct^2})
\end{equation}
It has been shown in \textit{2(a), p.29} that $[e^{tL},L]=0$. 
\begin{equation}
	\frac{d}{dt}G(t)=G(0)(e^{tB}e^{\frac{1}{2}ct^2})(B+ct)=G(t)(B+ct)
\end{equation}
\item
\begin{equation}
	G(1)\equiv e^{A+B}e^{-A}=G(0)e^Be^{c/2}
\end{equation}
\begin{equation}
	e^{A+B}=e^Be^Ae^{c/2}
\end{equation} 
Note that $[B,A]=-[A,B]$, thus $e^{A+B}=e^{B+A}=e^Ae^Be^{-c/2}$
\end{enumerate}
\end{sol}