\begin{sol}
Define the change of basis matrix
\begin{equation}
	S\equiv\frac{1}{\sqrt 2}\begin{pmatrix}
1&-1&0\\
0&0&\sqrt{2}\\
1&1&0
\end{pmatrix}\,\,\,\,\,S^{-1}\equiv\frac{1}{\sqrt 2}\begin{pmatrix}
1&0&1\\
-1&0&1\\
0&\sqrt{2}&0
\end{pmatrix}
\end{equation} 
In the new basis, 
\begin{equation}
	A_2=S^{-1}A_2S=\frac{1}{2}\begin{pmatrix}
1&0&1\\
-1&0&1\\
0&\sqrt{2}&0
\end{pmatrix}\begin{pmatrix}
2&1&1\\1&0&-1\\1&-1&2
\end{pmatrix}\begin{pmatrix}
1&-1&0\\
0&0&\sqrt{2}\\
1&1&0
\end{pmatrix}=\begin{pmatrix}
3&0&0\\
0&1&-\sqrt{2}\\
0&-\sqrt{2}&0
\end{pmatrix}
\end{equation} 
To find the eigenvalues, find the characteristic polynomial of $A_2$
\begin{equation}
	\det(A_2-\lambda\mathbf{1})=0
\end{equation} 
\begin{equation}
	\det\begin{pmatrix}
3-\lambda&0&0\\
0&1-\lambda&-\sqrt{2}\\
0&-\sqrt{2}&-\lambda
\end{pmatrix}=(3-\lambda)(-\lambda(1-\lambda)-2)=(3-\lambda)(\lambda-2)(\lambda+1)=0
\end{equation} 
\begin{equation}
	\lambda={3,2,-1}
\end{equation} 
\end{sol}