\begin{sol}
Note: $a$ will be used for $\Delta$ in the question to avoid confusion.
First, calculate the expectation values of $\hat x$ and $\hat p$
\begin{equation}
	\langle \hat x\rangle=\bra\Psi\hat x\ket\Psi=\int_{-\infty}^\infty \psi^*(x)x\psi(x)dx=\int_{-\infty}^\infty xe^{-\frac{x^2}{a^2}}dx=0
\end{equation} \begin{equation}
	\langle \hat p\rangle=\bra\Psi\hat p\ket\Psi=\int_{-\infty}^\infty\psi^*(x)\left(-i\frac{d}{dx}\right)\psi(x)dx=N^2\int_{-\infty}^\infty e^{-i\langle p\rangle x}e^{-\frac{x^2}{2a^2}}(-i)\left(i\langle p\rangle-\frac{x}{a}\right)e^{i\langle p\rangle x}e^{-\frac{x^2}{2a^2}}dx
\end{equation}  \begin{equation}
	=\langle p\rangle N^2\int_{-\infty}^\infty e^{-\frac{x^2}{a^2}}dx-\frac{iN^2}{a}\int_{-\infty}^\infty x e^{-\frac{x^2}{a^2}}dx=\langle p\rangle 
\end{equation} 
Substituting the operators into the condition for saturation will yield
\begin{equation}
	(\hat p-\langle p\rangle)\ket\Psi=i\gamma\hat x\ket\Psi
\end{equation} 
\begin{equation}
	-i\frac{d\psi(x)}{dx}-\langle p\rangle \psi(x)=i\gamma x\psi(x)
\end{equation} 
\begin{equation}
	\langle p\rangle N^2e^{i\langle p\rangle x}e^{-\frac{x^2}{2a^2}}+i\frac{x N^2}{a}e^{i\langle p\rangle x}e^{-\frac{x^2}{2a^2}}-\langle p\rangle N^2 e^{i\langle p\rangle x}e^{-\frac{x^2}{2a^2}}=i\gamma  N^2x e^{i\langle p\rangle x}e^{-\frac{x^2}{2a^2}}
\end{equation} 
\begin{equation}
	i\frac{x N^2}{a}e^{i\langle p\rangle x}e^{-\frac{x^2}{2a^2}}=i\gamma  N^2x e^{i\langle p\rangle x}e^{-\frac{x^2}{2a^2}}
\end{equation}


\begin{equation}
	\gamma=\frac{1}{a}
\end{equation} 
\end{sol}